another example in ERT

ERT.thy
@@ -29,18 +29,51 @@ primrec ert :: "hpgcl \<Rightarrow> (stack \<times> heap \<Rightarrow> ennreal) 
 | "ert (While b c) X = lfp (\<lambda>Y (s,h). 1 + (if b s then ert c Y (s,h) else X (s,h) ))" 
 | "ert (Assign v e) X = (\<lambda>(s,h). X (s(v:=e s),h) + 1)"
 
-| "ert (New x ve) X = (\<lambda>(s,h). Sup { ((emb\<^sub>p (ptb (\<lambda>_. a) ve))  -\<star>\<^sub>p (\<lambda>(s,h). X (s(x:=a),h))) (s,h) |a::int. a\<noteq>0 } + 1 )"
+| "ert (New x ve) X = (\<lambda>(s,h). Sup { (( (pt (\<lambda>_. a) ve))  -\<star>\<^sub>p (\<lambda>(s,h). X (s(x:=a),h))) (s,h) |a::int. a\<noteq>0 } + 1 )"
 | "ert (Free ae) X = (\<lambda>x. ((ptany ae) \<star>\<^sub>p X) x + 1)"
 | "ert (Lookup x ae) X =                             
-     (\<lambda>(s,h). Inf { ((pt ae (\<lambda>_. val)) \<star>\<^sub>p (emb\<^sub>p (ptb ae (\<lambda>_. val)) -\<star>\<^sub>p (\<lambda>(s,h). X (s(x:=val),h)))) (s,h)
+     (\<lambda>(s,h). Inf { ((pt ae (\<lambda>_. val)) \<star>\<^sub>p ( (pt ae (\<lambda>_. val)) -\<star>\<^sub>p (\<lambda>(s,h). X (s(x:=val),h)))) (s,h)
        |val::int. True } + 1)"
-| "ert (Update ae ve) X = (\<lambda>h. (ptany ae \<star>\<^sub>p ((emb\<^sub>p (ptb ae ve)) -\<star>\<^sub>p X)) h + 1)"
+| "ert (Update ae ve) X = (\<lambda>h. (ptany ae \<star>\<^sub>p (( (pt ae ve)) -\<star>\<^sub>p X)) h + 1)"
 
 
 
+
+
+lemma "(X \<star>\<^sub>p (\<lambda>_. 1)) = X + (\<lambda>_. 1)"
+  oops 
 
 
 subsection "example"
+
+
+(* for "garbage collection" *)
+definition "trueheap = (\<lambda>_. 0::ennreal)"
+           
+term sep_true
+
+lemma "trueheap = emb\<^sub>p (sep_true)" unfolding trueheap_def   emb\<^sub>p_alt by auto
+
+
+lemma GC: "trueheap \<le> X"  unfolding trueheap_def le_fun_def by auto
+lemma GC': "trueheap x \<le> X x"  unfolding trueheap_def le_fun_def by auto
+
+lemma addd_true_heaps: "((\<lambda>_. a) \<star>\<^sub>p (\<lambda>_. b)) = (\<lambda>_. a+b)"
+  apply (rule antisym)
+  unfolding star_pot_method_alt
+  subgoal apply(rule le_funI) apply (simp add: split_beta)
+    apply(rule Inf_lower) apply auto apply(rule exI[where x=0]) 
+    by(auto simp: sep_add_ac)
+  subgoal apply(rule le_funI) apply (simp add: split_beta) 
+    apply(rule Inf_greatest) by auto
+  done
+
+
+lemma adjoint_general_s'':
+  "Y \<le> (X \<star>\<^sub>p Z) \<Longrightarrow> (Z -\<star>\<^sub>p Y) sh  \<le> X sh"
+  using adjoint_general_s' unfolding le_fun_def by fast
+
+
 
 experiment
 begin
@@ -65,11 +98,81 @@ lemma "ert P (\<lambda>_. 0) x \<le> 2"
   apply(cases x) apply auto
   apply(rule SUP_least) by simp  
 
+lemma "(Sup A) x = Sup ((\<lambda>a. a x) ` A)"
+  by simp
+
+lemma pp: "(\<lambda>x. (Sup A) x) = (\<lambda>x. Sup ((\<lambda>a. a x) ` A))"
+  by simp
 
 
+lemma "ert P (\<lambda>_. 0)  \<le> (\<lambda>_. 2)"
+  unfolding P_def 
+  apply(subst ert.simps)
+  apply(subst ert.simps)
+  apply(subst ert.simps)
+  apply(rule le_funI)
+  apply(simp add: split_beta)
+  apply (auto simp: algebra_simps)
+  apply(subst f) apply(rule Sup_least)
+  apply auto  
+  apply(rule adjoint_general_s'')
 
+  apply auto
+  apply(rule le_funI)
+  apply(rule order.trans)
+   defer apply(rule star_pot_method_mono[where B="(\<lambda>_.1)"])
+    defer 
+      apply(rule GC'[where X="emb\<^sub>p (ptb (\<lambda>_. _) (\<lambda>_. 1))"])
+   defer  apply simp 
+  unfolding trueheap_def 
+  apply(subst addd_true_heaps) by auto 
+   
 
 end
+
+
+experiment
+begin
+
+definition P where "P = Seq (New ''a'' (\<lambda>_. 1)) (Coin Skip (0.5) (Lookup ''b'' (\<lambda>s. s ''a'')))"
+
+
+lemma f: "1+l\<le>2 \<longleftrightarrow> l\<le>(1::ennreal)"
+  apply rule 
+  subgoal by (metis ennreal_add_left_cancel_le infinity_ennreal_def one_add_one top.extremum)  
+  subgoal by (metis ennreal_add_left_cancel_le one_add_one)
+  done
+
+
+lemma "ert P (\<lambda>_. 0) x \<le> 2"
+  unfolding P_def 
+  apply(subst ert.simps)
+  apply(subst ert.simps)
+  apply(subst ert.simps)
+  apply(subst ert.simps)
+  apply(subst ert.simps) 
+  apply(simp add: split_beta)
+  apply (auto simp: algebra_simps)
+  apply(subst f) apply(rule Sup_least)
+  apply auto
+  apply(rule order.trans)
+  apply(rule wand_pot_method_Rmono) 
+   apply(simp add: split_beta)
+  apply(rule add_left_mono)
+  apply(rule add_left_mono)
+   apply(rule mult_left_mono) 
+    apply(rule Inf_mono[where B="{uu. \<exists>val. uu = ((\<lambda>(s, h). 0)) ((fst _)(''a'' := _), snd _)}"]) 
+  apply simp
+
+
+  thm quant_modus_ponens_general_s
+
+
+
+  apply(rule adjoint_general_s'')
+  apply(simp add: split_beta)
+  apply auto oops
+
 
 
 end
